messageInvariantPrototypes/ringLeaderElection/monotonic/hosts.dfy
@@ -1,0 +1,104 @@
+include "../../lib/UtilitiesLibrary.dfy"
+
+module Types {
+  import opened UtilitiesLibrary
+
+  type HostId = nat
+
+  datatype Message = Msg(val: nat, src: nat)  // A host can receive if its ringPos == succ(src)
+
+  datatype MessageOps = MessageOps(recv:Option<Message>, send:Option<Message>)
+} // end module Types
+
+
+module Host {
+  import opened UtilitiesLibrary
+  import opened Types
+
+  datatype Constants = Constants(numParticipants:nat, ringPos: nat, hostId: HostId)
+
+  predicate ConstantsValidForGroup(c: Constants, participantCount: nat, ringPos: HostId)
+  {
+    && c.numParticipants == participantCount
+    && c.ringPos == ringPos
+  }
+
+  datatype Variables = Variables(
+    highestHeardSeq: seq<nat>
+  )
+  {
+    predicate WF(c: Constants) {
+      && 0 < c.numParticipants
+    }
+
+    function highestHeard(): int {
+      if highestHeardSeq == [] then -1
+      else Last(highestHeardSeq)
+    }
+  }
+
+  predicate GroupWFConstants(grp_c: seq<Constants>) {
+    && 0 < |grp_c|
+    && (forall ringPos: nat | ringPos < |grp_c|
+        :: ConstantsValidForGroup(grp_c[ringPos], |grp_c|, ringPos))
+  }
+
+  predicate GroupWF(grp_c: seq<Constants>, grp_v: seq<Variables>) {
+    && GroupWFConstants(grp_c)
+    // Variables size matches group size defined by grp_c
+    && |grp_v| == |grp_c|
+    // Each host is well-formed
+    && (forall i | 0 <= i < |grp_c| :: grp_v[i].WF(grp_c[i]))
+  }
+
+  predicate GroupInit(grp_c: seq<Constants>, grp_v: seq<Variables>) {
+    && GroupWF(grp_c, grp_v)
+    && (forall i | 0 <= i < |grp_c| :: Init(grp_c[i], grp_v[i]))
+  }
+
+  predicate Init(c: Constants, v: Variables)
+  {
+    && v.WF(c)
+    && v.highestHeardSeq == []
+  }
+
+  datatype Step =
+    TransmissionStep() | ReceiveStep()
+
+  predicate NextStep(c: Constants, v: Variables, v': Variables, step: Step, msgOps: MessageOps)
+  {
+    && v.WF(c)
+    && match step
+      case TransmissionStep => NextTransmissionStep(c, v, v', msgOps)
+      case ReceiveStep => NextReceiveStep(c, v, v', msgOps)
+  }
+
+  predicate NextTransmissionStep(c: Constants, v: Variables, v': Variables, msgOps: MessageOps) 
+    requires v.WF(c)
+  {
+    var payload := max(v.highestHeard(), c.hostId); // max of what I heard vs my own hostId
+    var msg := Msg(payload, c.ringPos);
+    && msgOps.recv.None?
+    && msgOps.send == Some(msg)
+    && v == v'
+  }
+
+  predicate NextReceiveStep(c: Constants, v: Variables, v': Variables, msgOps: MessageOps) {
+    && msgOps.send.None?
+    && msgOps.recv.Some?
+    && msgOps.recv.value.src < c.numParticipants
+    && c.ringPos == Successor(c.numParticipants, msgOps.recv.value.src)
+    && if msgOps.recv.value.val >= v.highestHeard() then 
+          v' == v.(highestHeardSeq := v.highestHeardSeq + [msgOps.recv.value.val])
+       else
+          v' == v
+  }
+
+  predicate Next(c: Constants, v: Variables, v': Variables, msgOps: MessageOps)
+  {
+    exists step :: NextStep(c, v, v', step, msgOps)
+  }
+}  // end module Host
+
+
+
